template-coq/theories/EnvironmentTyping.v
@@ -22,7 +22,7 @@ Module Lookup (T : Term) (E : EnvironmentSig T).
     declared_inductive Σ (fst cstr) mdecl idecl /\
     List.nth_error idecl.(ind_ctors) (snd cstr) = Some cdecl.
 
-  Definition declared_projection Σ mdecl idecl (proj : projection) pdecl
+  Definition declared_projection Σ (proj : projection) mdecl idecl pdecl
   : Prop :=
     declared_inductive Σ (fst (fst proj)) mdecl idecl /\
     List.nth_error idecl.(ind_projs) (snd proj) = Some pdecl /\
