pcuic/theories/PCUICInversion.v
@@ -194,7 +194,7 @@ Section Inversion.
     forall {Γ p c T},
       Σ ;;; Γ |- tProj p c : T ->
       ∑ u mdecl idecl pdecl args,
-        declared_projection Σ mdecl idecl p pdecl ×
+        declared_projection Σ p mdecl idecl pdecl ×
         Σ ;;; Γ |- c : mkApps (tInd (fst (fst p)) u) args ×
         #|args| = ind_npars mdecl ×
         let ty := snd pdecl in
