pcuic/theories/PCUICTyping.v
@@ -288,7 +288,7 @@ Inductive typing `{checker_flags} (Σ : global_env_ext) (Γ : context) : term ->
 
 | type_Proj p c u :
     forall mdecl idecl pdecl,
-    declared_projection Σ.1 mdecl idecl p pdecl ->
+    declared_projection Σ.1 p mdecl idecl pdecl ->
     forall args,
     Σ ;;; Γ |- c : mkApps (tInd (fst (fst p)) u) args ->
     #|args| = ind_npars mdecl ->
@@ -679,7 +679,7 @@ Lemma typing_ind_env_app_size `{cf : checker_flags} :
         P Σ Γ (tCase ci p c brs) (mkApps ptm (indices ++ [c]))) ->
 
    (forall Σ (wfΣ : wf Σ.1) (Γ : context) (wfΓ : wf_local Σ Γ) (p : projection) (c : term) u
-         mdecl idecl pdecl (isdecl : declared_projection Σ.1 mdecl idecl p pdecl) args,
+         mdecl idecl pdecl (isdecl : declared_projection Σ.1 p mdecl idecl pdecl) args,
        Forall_decls_typing P Σ.1 -> PΓ Σ Γ wfΓ ->
        Σ ;;; Γ |- c : mkApps (tInd (fst (fst p)) u) args ->
        P Σ Γ c (mkApps (tInd (fst (fst p)) u) args) ->
@@ -1085,7 +1085,7 @@ Lemma typing_ind_env `{cf : checker_flags} :
           
 
     (forall Σ (wfΣ : wf Σ.1) (Γ : context) (wfΓ : wf_local Σ Γ) (p : projection) (c : term) u
-          mdecl idecl pdecl (isdecl : declared_projection Σ.1 mdecl idecl p pdecl) args,
+          mdecl idecl pdecl (isdecl : declared_projection Σ.1 p mdecl idecl pdecl) args,
         Forall_decls_typing P Σ.1 -> PΓ Σ Γ wfΓ ->
         Σ ;;; Γ |- c : mkApps (tInd (fst (fst p)) u) args ->
         P Σ Γ c (mkApps (tInd (fst (fst p)) u) args) ->
